inference-tool/src/main/python/test.py
@@ -1,0 +1,117 @@
+#!/usr/bin/env python3
+# -*- coding: utf-8 -*-
+"""
+Created on Fri Apr 29 08:13:14 2022
+
+@author: michael
+"""
+from deap import gp
+from deap import creator
+from deap import base
+
+import operator
+import networkx as nx
+import z3
+
+creator.create("FitnessMin", base.Fitness, weights=(-1.0,))
+creator.create("Individual", gp.PrimitiveTree, fitness=creator.FitnessMin)
+
+
+def to_z3(tree, labels, types):
+    def _make_tuple(tree, root, _parent):
+        # Get the neighbors of `root` that are not the parent node. We
+        # are guaranteed that `root` is always in `tree` by construction.
+        children = set(tree[root]) - {_parent}
+        if len(children) == 0:
+            if labels[root] in types:
+                return types[labels[root]](labels[root])
+            else:
+                return labels[root]
+
+        nested = tuple(_make_tuple(tree, v, root) for v in children)
+        if labels[root] == "add":
+            c1, c2 = nested
+            return c1 + c2
+        elif labels[root] == "sub":
+            c1, c2 = nested
+            return c1 - c2
+        elif labels[root] == "mul":
+            c1, c2 = nested
+            return c1 * c2
+        elif labels[root] == "div":
+            c1, c2 = nested
+            try:
+                return c1 / c2
+            except ZeroDivisionError:
+                return float("inf")
+        elif labels[root] == "id":
+            return nested[0]
+        else:
+            raise ValueError(f"Invalid operator {root}")
+
+    # Do some sanity checks on the input.
+    root = 0  # By construction of GP individuals
+    if not nx.is_tree(tree):
+        raise nx.NotATree("provided graph is not a tree")
+    if root not in tree:
+        raise nx.NodeNotFound(f"Graph {tree} contains no node {root}")
+
+    return _make_tuple(tree, root, None)
+
+
+def make_binary(fun, children):
+    if len(children) == 2:
+        c1 = to_exp_string(children[0])
+        c2 = to_exp_string(children[1])
+        return f"{fun}({c1}, {c2})"
+    else:
+        c1 = to_exp_string(children[0])
+        c2 = make_binary(fun, children[1:])
+        return f"{fun}({c1}, {c2})"
+
+
+def to_exp_string(exp):
+    if str(exp.decl()) == "+":
+        return make_binary("add", exp.children())
+    elif str(exp.decl()) == "-":
+        return make_binary("sub", exp.children())
+    elif str(exp.decl()) == "*":
+        return make_binary("mul", exp.children())
+    elif str(exp.decl()) == "/":
+        return make_binary("div", exp.children())
+    elif type(exp) == z3.RatNumRef:
+        x2 = exp.as_fraction()
+        return str(float(x2.numerator) / float(x2.denominator))
+    else:
+        return str(exp)
+
+
+def from_z3(exp, pset):
+    return gp.PrimitiveTree.from_string(to_exp_string(exp), pset)
+
+
+def simplify(individual, pset, types):
+    # Duplicate the individual
+    individual = creator.Individual(gp.PrimitiveTree.from_string(str(individual), pset))
+    nodes, edges, labels = gp.graph(individual)
+    g = nx.Graph()
+    g.add_nodes_from(nodes)
+    g.add_edges_from(edges)
+
+    z3_exp = to_z3(g, labels, types)
+    print(z3_exp)
+    if type(z3_exp) in {int, float, str}:
+        return creator.Individual(gp.PrimitiveTree([gp.Terminal(z3_exp)]))
+    return creator.Individual(from_z3(z3.simplify(z3_exp), pset))
+
+
+pset = gp.PrimitiveSetTyped("MAIN", [int], int)
+pset.renameArguments(ARG0="r1")
+pset.addPrimitive(operator.add, [int, int], int)
+pset.addPrimitive(operator.sub, [int, int], int)
+pset.addPrimitive(operator.mul, [int, int], int)
+
+seed = "add(mul(0, 0), sub(r1, 50))"
+exp = gp.PrimitiveTree.from_string(seed, pset)
+simplified = simplify(exp, pset, {'r1': z3.Int})
+print(simplified)
