formal/Extended_Finite_State_Machines/Show_EFSM.thy
@@ -1,0 +1,23 @@
+theory Show_EFSM
+imports EFSM Show.Show_Instances
+begin
+
+
+lemma "show 5 = ''5''"
+  apply (simp add: shows_prec_nat_def)
+  oops
+
+instantiation "value" :: "show" begin
+fun showsp_value :: "value showsp" where
+  "showsp_value p (value.Int a) = shows_string (show a)" |
+  "showsp_value p (value.Str a) = shows_string (String.explode a)" |
+  "showsp_value p (value.Real a) = shows_string ''a''"
+
+instance
+  apply standard
+  subgoal for p x r s
+    apply (induct x)
+
+end
+
+end
